# 例题部分

## 极限

> **证明:**
>
> 1. 证明:$\lim_{x\to x_0}x=x_0$
> 2. 证明:$\lim_{x\to x_0}c=c$
> 3. 证明:$\lim_{x\to x_0}\sqrt{x}=\sqrt{x_0}$
> 4. 证明:$\lim_{x\to\infty}\frac{1}{x}=0$
> 5. 证明:$\lim_{x\to x_0}f(x)=\infty为无穷大,\lim_{x\to x_0}\frac{1}{f(x)}=0为无穷小$
> 6. 证明:$\lim[f(x)\pm g(x)]=\lim f(x) \pm \lim g(x).$
> 7. 证明:$\lim[f(x)\cdot g(x)]=\lim f(x) \cdot \lim g(x).$
> 8. 证明:$\lim\frac{f(x)}{g(x)}=\frac{\lim f(x)}{\lim g(x)},(\lim g(x)\not=0)$
> 9. 证明:$\lim_{x \to 0}\frac{\sin x}{x}=1,\lim_{x \to 0}\cos x=1$
> 10. 证明:$\lim_{x\to \infty}(1+\frac{1}{x})^x=e$
> 11. 证明:$当x\to0$,	$ \sin x$~$x$,	$\tan x$~$x$	$\arcsin x$~$x$,    $1-\cos x$~$\frac{1}{2}x^2$
> 12. 证明:$当x\to0, \sqrt[n]{1+x}-1$~$\frac{1}{n}x$
> 13. 证明:当$x\to0,\ln(1+x)$~ $x , e^x-1$~ $x,(1+x)^\alpha-1$~ $\alpha x$.

> **极限:**
>
> 1. 求:$\lim_{x\to0}\frac{\tan x}{x}=1$
> 2. 求:$\lim_{x\to0}\frac{1-\cos x}{x^2}=\frac{1}{2}$
> 3. 求:$\lim_{x\to0}\frac{\arcsin x}{x}=1$
> 4. 求:$\lim_{x\to \infty}(1-\frac{1}{x})^x=\frac{1}{e}$
> 5. 求:$\lim_{x\to3}\sqrt{\frac{x-3}{x-9}}=\frac{\sqrt{6}}{6}.$
> 6. 求:$\lim_{x\to0}\frac{\log_a(1+x)}{x}=\frac{1}{\ln a}$
> 7. 求:$\lim_{x\to0}\frac{a^x-1}{x}=\ln a$
> 8. 求:$\lim_{x\to0}\frac{(1+x)^\alpha-1}{x}=\alpha$
> 9. 求:$\lim_{x\to0}(1+2x)^\frac{3}{\sin x}=e^6$

> **例题:**
>
> - 证明:$\lim_{x \to 1}(2x-1)=1$
> - 证明:$\lim_{x\to 1}\frac{x^2-1}{x-1}=2$
> - 求左右极限:$f(x) = \begin{cases} x-1, &  x<0 \\ 0, & x=0\\ x+1,&x > 0 \end{cases},\to \\\lim_{x\to0^-}f(x)=\lim_{x\to0^-}(x-1)=-1,\lim_{x\to0^+}f(x)=\lim_{x\to0^+}(x-1)=1$
> - 证明$\lim_{x\to1}\frac{1}{x-1}=\infty$
> - 求:$\lim_{x\to 1}(2x-1)=1$
> - 求:$\lim_{x\to2}\frac{x^3-1}{x^2-5x+3}=-\frac{7}{3}$
> - 求:$\lim_{x\to 3}\frac{x-3}{x^2-9}=\frac{1}{6}$
> - 求:$\lim_{x\to 1}\frac{2x-3}{x^2-5x+4}=\infty$
> - 求:$\lim_{x\to \infty}\frac{3x^3+4x^2+2}{7x^3+5x^2-3}=\frac{3}{7}$
> - 求:$\lim_{x\to \infty}\frac{3x^2-2x-1}{2x^3-x^2+5}=0$
> - 求:$\lim_{x\to \infty}\frac{2x^3-x^2+5}{3x^2-2x-1}=\infty$
> - 求:$\lim_{x\to \infty}\frac{\sin x}{x}=0$
> - 求:$\lim_{x\to0}\frac{\tan 2x}{\sin 5x}=\frac{2}{5}$
> - 求:$\lim_{x\to0}\frac{\sin x}{x^3+3x}=\frac{1}{3}$
> - 求:$\lim_{x\to0}\frac{(1+x^2)^\frac{1}{3}-1}{\cos x-1}=-\frac{2}{3}$.

## 导数

> **证明:**
>
> 1. 证明:$[u(x)\pm v(x)]'=u'(x)\pm v'(x)$
> 2. 证明:$[u(x)v(x)]'=u'(x)v(x)+u(x)v'(x)$
> 3. 证明:$[(\frac{u(x)}{v(x)})]'=\frac{u'(x)v(x)-u(x)v'(x)}{v^2(x)}(v(x)\not=0)$
> 4. 证明:$(Cu)'=Cu'$
> 5. 证明:$[f^{-1}(x)]'=\frac{1}{f'(y)},\frac{dy}{dx}=\frac{1}{\frac{dx}{dy}}.$
> 6. 证明:$\frac{dy}{dx}=\frac{dy}{du}\cdot\frac{du}{dt}$
> 7. 证明:$(u\pm v)^{(n)}=u^{(n)}\pm v^{(n)}$
> 8. 证明:$(uv)^{(n)}=\sum_{k=0}^nC^k_nu^{(n-k)}v^{(k)}.$
> 9. 证明:$\begin{cases} x=\varphi(t)\\y=\psi(t) \end{cases},\to\frac{dy}{dx}=\frac{\psi'(t)}{\varphi'(t)}.$

> **导数:**
>
> 1. 求:$f(x)=C\to (C)'=0$
> 2. 求:$f(x)=x^n(n\in N_+) \to (x^n)'=\begin{cases} 1,n=1\\nx^{n-1},n>1 \end{cases}$
> 3. 求:$f(x)=x^\mu(\mu \in R)\to (x^\mu)'=\mu x^{\mu-1}$
> 4. 求:$f(x)=\sin x\to (\sin x)'=\cos x,(\cos x)'=-\sin x$
> 5. 求:$f(x)=a^x(a>0,a\not=1)\to (a^x)'=a^x\ln a,(e^x)'=e^x$
> 6. 求:$f(x)=\log_ax(a>0,a\not=1)\to(\log_ax)'=\frac{1}{x\ln a},(\ln x)'=\frac{1}{x}$
> 7. 求:$y=\frac{1}{x},在(\frac{1}{2},2)$处的切线斜率 $y'=-\frac{1}{x^2}$
> 8. 求:$y=ax+b, \to y'=a, y''=0$
> 9. 求:$s=sin\omega t,\to s'=\omega cos\omega t,s''=-\omega^2\sin\omega t.$
> 10. 求:$y=e^x ,\to (e^x)^{(n)}=e^x$
> 11. 求:$y=\sin x,\to y'=\cos x=\sin(\frac{x+\pi}{2}),(\sin x)^{(n)}=sin(x+n\cdot\frac{\pi}{2}),(\cos x)^{(n)}=cos(x+n\cdot\frac{\pi}{2})$
> 12. 求:$y=\ln(x+1),\to y'=\frac{1}{1+x},y''=-\frac{1}{(1+x)^2},y'''=\frac{1\cdot2}{(1+x)^3},y^{(n)}=(-1)^{n-1}\frac{(n-1)!}{(1+x)^n}.$
> 13. 求:$y=x^\mu,\to y'=\mu x^{\mu-1},y''=\mu(\mu-1)x^{\mu-2},y^{(n)}=\mu(\mu-1)(\mu-2)(\mu-3)...(\mu-n+1)x^{\mu-n}.$
> 14. 求:$y=x^2e^{2x},\to求y^{(20)}\to \\ u^{(k)}=2^ke^{2x}(k=1,2,3,...),v'=2x,v''=2,v^{(k)}=0(k=3,4,...)\\ y^{(20)}=2^{20}e^{2x}(x^2+20x+95)$
> 15. 求:$e^y+xy-e=0 \to \frac{dy}{dx}=-\frac{y}{x+e^y}$
> 16. 求:$y=x^{\sin x}(x>0),\to y'=x^{\sin x}(\cos x\cdot \ln x+\frac{\sin x}{x}).$
> 17. 求:$y=\sqrt{\frac{(x-1)(x-2)}{(x-3)(x-4)}},\to y'=\frac{y}{2}(\frac{1}{x-1}+\frac{1}{x-2}+\frac{1}{x-3}+\frac{1}{x-4}).$
> 18. 求:$\begin{cases} x=a\cos t\\y=b\sin t \end{cases},\to\frac{dy}{dx}=-\frac{b}{a}.$
> 19. 求:$\begin{cases} x=v_1t\\y=v_2-\frac{1}{2}gt^2 \end{cases},\to\frac{dy}{dx}=\frac{v_2-gt}{v_1}.$
> 20. 求:$\begin{cases} x=a(t-\sin t)\\y=b(1-\cos t) \end{cases},\to \frac{dy}{dx}=\cot\frac{t}{2},\to \frac{d^2y}{dx^2}=-\frac{1}{a(1-\cos t)^2}.$
> 21. 求:$\tan \alpha=\frac{h}{500},对t求导,\to \sec^2\alpha\cdot\frac{d\alpha}{dt}=\frac{1}{500}\cdot\frac{dh}{dt}.$

> **例题:**
>
> - 求:$f(x)=|x|在x=0$处的导数.$\begin{cases} \lim_{h\to0^-}\frac{|h|}{h}=-1\\\lim_{h\to0^+}\frac{|h|}{h}=1\end{cases}$左右导数不相等,故在$x=0$处不可导.
> - 求:$f(x)=\sqrt[3]{x}$在区间$(-\infty,+\infty)$内连续,但在,点$x=0$处不可导(或者称导数为无穷大其实为几何图形中垂直于$x$轴的切线$x=0$),$\lim_{h\to0}\frac{f(0+h)-f(0)}{h}=\lim_{h\to0}\frac{1}{h^{\frac{2}{3}}}=+\infty$.
> - 求:$y=2x^3-5x^2+3x-7\to y'=6x^2-10x+3$
> - 求:$y=x^3+4\cos x-sin\frac{\pi}{2} \to y'=3x^2-4\sin x$
> - 求:$y=e^x(\sin x+\cos x)\to y'=2e^x\cos x$
> - 求:$y=\tan x\to y'=\sec^2x$
> - 求:$y=\sec x\to y'=\sec x\tan x$
> - 求:$(\cot x)'=-\csc^2x,(\csc x)'=-\csc x\cot x$
> - 求:$y=\arcsin x \to y'=\frac{1}{\sqrt(1-x^2)}$
> - 求:$y=\arccos x \to y'=-\frac{1}{\sqrt(1-x^2)}$
> - 求:$y=\arctan x \to y'=\frac{1}{1+x^2}$
> - 求:$y=arccot x \to y'=-\frac{1}{1+x^2}$
> - 求:$y=e^{x^3}\to\frac{dy}{dx}=3x^2e^{x^3}$
> - 求:$y=\sin \frac{2x}{1+x^2} \to\frac{dy}{dx}=\frac{2(1-x^2)}{(1+x^2)^2}\cdot\cos\frac{2x}{1+x^2}$
> - 求:$y=\ln \sin x\to \frac{dy}{dx}=\cot x$
> - 求:$y=\sqrt[3]{1-2x^2}\to \frac{dy}{dx}=\frac{-4x}{3\sqrt[3]{(1-2x^2)^2}}$
> - 求:$y=\ln \cos(e^x) \to \frac{dy}{dx}=-e^x\tan(e^x)$
> - 求:$y=e^{\sin\frac{1}{x}} \to \frac{dy}{dx}=-\frac{1}{x^2}e^{\sin\frac{1}{x}}\cdot\cos\frac{1}{x}.$
> - 求:$y=\sin nx\cdot\sin^nx \to \frac{dy}{dx}=n\sin^{n-1}x\cdot\sin(n+1)x$
> - 求:$(shx)'=chx,(chx)'=shx,(thx)'=\frac{1}{ch^2x}$
> - 求:$(arshx)'=\frac{1}{\sqrt{1+x^2} },(archx)'=\frac{1}{\sqrt{x^2-1}},(arthx)'=\frac{1}{1-x^2}$
> - 求:$y^5+2y-x-3x^7=0,\to \frac{dy}{dx}=\frac{1+21x^6}{5y^4+2}$
> - 求:$\frac{x^2}{16}+\frac{y^2}{9}=1,\to \frac{dy}{dx}=-\frac{9x}{16y}$
> - 求:$x-y+\frac{1}{2}\sin y=0,\to\frac{dy}{dx}=\frac{2}{2-\cos y},\to \frac{d^2y}{dx^2}=\frac{-4\sin y}{(2-\cos y)^3}$